Wip on Encrypt path

src/SDK/MessageBody.dfy
@@ -3,55 +3,39 @@
 
 include "../StandardLibrary/StandardLibrary.dfy"
 include "../StandardLibrary/UInt.dfy"
-include "MessageHeader.dfy"
 include "Serialize/SerializableTypes.dfy"
 include "../AwsCryptographicMaterialProviders/Client.dfy"
 include "../Crypto/AESEncryption.dfy"
 include "../Util/Streams.dfy"
 include "../Util/UTF8.dfy"
+include "Serialize/Frames.dfy"
+
+include "Serialize/Header.dfy"
+include "Serialize/HeaderTypes.dfy"
+include "Serialize/V1HeaderBody.dfy"
+include "Serialize/HeaderAuth.dfy"
+include "../../libraries/src/Collections/Sequences/Seq.dfy"
+
 
 module MessageBody {
-  export
-    provides EncryptMessageBody, DecryptFramedMessageBody, DecryptNonFramedMessageBody,
-      Wrappers, UInt, Msg, Streams, FramesToSequence, Client,
-      FrameToSequence, ValidFrames, FramesEncryptPlaintext, AESEncryption, DecryptedWithKey
-    reveals Frame, Frame.Valid, SeqWithGhostFrames
+  // export
+  //   provides EncryptMessageBody, DecryptFramedMessageBody, DecryptNonFramedMessageBody,
+  //     Wrappers, UInt, Streams, Client,
+  //     FramesEncryptPlaintext, AESEncryption, DecryptedWithKey
+  //   reveals  SeqWithGhostFrames
 
   import opened Wrappers
   import opened UInt = StandardLibrary.UInt
-  import Msg = MessageHeader
   import AESEncryption
   import Streams
   import UTF8
   import SerializableTypes
   import MaterialProviders.Client
+  import Frames
+  import Header
+  import Seq
 
   datatype BodyAADContent = AADRegularFrame | AADFinalFrame | AADSingleBlock
-
-  /**
-    The behavior of the methods in this file are specified in https://github.com/awslabs/aws-encryption-sdk-specification/blob/master/data-format/message-body.md
-    The Frame datatype has been introduced in the validation of this file. This datatype is only used for the validation.
-    The methods in this file serialize and deserialize some plaintext to frames. Frame are encoded in a sequence of bytes.
-  */
-
-  // Predicate all conditions which should hold for any valid sequence of frames
-  predicate ValidFrames(frames: seq<Frame>) {
-    0 < |frames| < UINT32_LIMIT &&
-    forall i | 0 <= i < |frames| ::
-      var frame := frames[i];
-      frame.Valid() &&
-      (if i == |frames| - 1 then frame.FinalFrame? else frame.RegularFrame?) &&
-      frame.seqNum as int == i + START_SEQUENCE_NUMBER as int &&
-      (forall j | i < j < |frames| :: frame.iv != frames[j].iv)
-  }
-
-  datatype Frame = RegularFrame(seqNum: uint32, iv: seq<uint8>, encContent: seq<uint8>, authTag: seq<uint8>) |
-                   FinalFrame(seqNum: uint32, iv: seq<uint8>, encContent: seq<uint8>, authTag: seq<uint8>)
-  {
-    predicate Valid() {
-      |encContent| < UINT32_LIMIT
-    }
-  }
 
   const BODY_AAD_CONTENT_REGULAR_FRAME: string := "AWSKMSEncryptionClient Frame"
   const BODY_AAD_CONTENT_FINAL_FRAME: string := "AWSKMSEncryptionClient Final Frame"
@@ -68,13 +52,18 @@ module MessageBody {
   const ENDFRAME_SEQUENCE_NUMBER: uint32 := 0xFFFF_FFFF
   const NONFRAMED_SEQUENCE_NUMBER: uint32 := 1
 
-  function method IVSeq(suite: Client.AlgorithmSuites.AlgorithmSuite, sequenceNumber: uint32): seq<uint8> {
+  function method IVSeq(suite: Client.AlgorithmSuites.AlgorithmSuite, sequenceNumber: uint32)
+    :(ret: seq<uint8>)
+    // The suite dictates the length of the IV
+    // this relationship is useful for correctness
+    ensures |ret| == suite.encrypt.ivLength as nat
+  {
     seq(suite.encrypt.ivLength as int - 4, _ => 0) + UInt32ToSeq(sequenceNumber)
   }
 
   lemma IVSeqDistinct(suite: Client.AlgorithmSuites.AlgorithmSuite, m: uint32, n: uint32)
     requires m != n
-    ensures 
+    ensures
       var algorithmSuiteID := SerializableTypes.GetESDKAlgorithmSuiteId(suite.id);
       && IVSeq(suite, m) != IVSeq(suite, n)
   {
@@ -85,44 +74,6 @@ module MessageBody {
     UInt32SeqSerializeDeserialize(n);
   }
 
-  // Converts sequence of Frames to a sequence encoding all frames
-  function FramesToSequence(frames : seq<Frame>): seq<uint8>
-    requires forall frame | frame in frames :: frame.Valid()
-  {
-    if frames == [] then
-      []
-    else
-      FramesToSequence(frames[..|frames| - 1]) + FrameToSequence(frames[|frames| - 1])
-  }
-
-  lemma ExtendFramesToSequence(frames: seq<Frame>, frame: Frame)
-    requires |frames| < UINT32_LIMIT - 1
-    requires forall frame | frame in frames :: frame.Valid()
-    requires frame.Valid()
-    ensures FramesToSequence(frames + [frame]) == FramesToSequence(frames) + FrameToSequence(frame)
-  {
-  }
-
-  // Converts Frame to a sequence encoding a frame
-  function FrameToSequence(frame: Frame): (res: seq<uint8>)
-    requires frame.Valid()
-    ensures match frame
-      case RegularFrame(_, iv: seq<uint8>, encContent: seq<uint8>, authTag: seq<uint8>) =>
-        4 + |iv| + |encContent| + |authTag| == |res|
-      case FinalFrame(seqNum: uint32, iv: seq<uint8>, encContent: seq<uint8>, authTag: seq<uint8>) =>
-        4 + 4 + |iv| + 4 + |encContent| + |authTag| == |res|
-  {
-    match frame
-      case RegularFrame(seqNum, iv, encContent, authTag) =>
-        var seqNumSeq := UInt32ToSeq(seqNum);
-        seqNumSeq + iv + encContent + authTag
-      case FinalFrame(seqNum, iv, encContent, authTag) =>
-        var seqNumEndSeq := UInt32ToSeq(ENDFRAME_SEQUENCE_NUMBER);
-        var seqNumSeq := UInt32ToSeq(seqNum);
-        var encContentLengthSeq := UInt32ToSeq(|encContent| as uint32);
-        seqNumEndSeq + seqNumSeq + iv + encContentLengthSeq + encContent + authTag
-  }
-
   /**
     Predicate states that frames encrypt plaintext
 
@@ -130,13 +81,15 @@ module MessageBody {
         FramesEncryptPlaintextSegments: States that sequence of frames decrypts to sequence of chunks
         SumPlaintextSegments: States that sum of chunks is the plaintext
    */
-  predicate FramesEncryptPlaintext(frames: seq<Frame>, plaintext: seq<uint8>)
+  predicate FramesEncryptPlaintext(frames: FramedMessage, plaintext: seq<uint8>)
   {
-    exists plaintextSeg: seq<seq<uint8>> ::
-      FramesEncryptPlaintextSegments(frames, plaintextSeg) && SumPlaintextSegments(plaintextSeg) == plaintext
+    exists plaintextSeg: seq<seq<uint8>>
+    ::
+    && FramesEncryptPlaintextSegments(frames, plaintextSeg)
+    && SumPlaintextSegments(plaintextSeg) == plaintext
   }
 
-  predicate FramesEncryptPlaintextSegments(frames: seq<Frame>, plaintextSeg: seq<seq<uint8>>)
+  predicate FramesEncryptPlaintextSegments(frames: FramedMessage, plaintextSeg: seq<seq<uint8>>)
   {
     if |frames| != |plaintextSeg| then
       false
@@ -144,17 +97,17 @@ module MessageBody {
       if frames == [] then
         true
       else
-        FramesEncryptPlaintextSegments(frames[..|frames| - 1], plaintextSeg[..|frames| - 1]) &&
-        AESEncryption.CiphertextGeneratedWithPlaintext(frames[|frames| - 1].encContent, plaintextSeg[|frames| - 1])
+        && FramesEncryptPlaintextSegments(frames[..|frames| - 1], plaintextSeg[..|frames| - 1])
+        && AESEncryption.CiphertextGeneratedWithPlaintext(frames[|frames| - 1].encContent, plaintextSeg[|frames| - 1])
   }
 
-  // Steps for inductive proofs EncryptMessageBody
-  lemma ExtendFramesEncryptPlaintextSegments(frames: seq<Frame>, plaintextSeg: seq<seq<uint8>>, frame: Frame, plaintextFrame: seq<uint8>)
-    requires FramesEncryptPlaintextSegments(frames, plaintextSeg)
-    requires AESEncryption.CiphertextGeneratedWithPlaintext(frame.encContent, plaintextFrame)
-    ensures FramesEncryptPlaintextSegments(frames + [frame], plaintextSeg + [plaintextFrame])
-  {
-  }
+  // // Steps for inductive proofs EncryptMessageBody
+  // lemma ExtendFramesEncryptPlaintextSegments(frames: seq<Frame>, plaintextSeg: seq<seq<uint8>>, frame: Frame, plaintextFrame: seq<uint8>)
+  //   requires FramesEncryptPlaintextSegments(frames, plaintextSeg)
+  //   requires AESEncryption.CiphertextGeneratedWithPlaintext(frame.encContent, plaintextFrame)
+  //   ensures FramesEncryptPlaintextSegments(frames + [frame], plaintextSeg + [plaintextFrame])
+  // {
+  // }
 
   function SumPlaintextSegments(plaintextSeg: seq<seq<uint8>>): seq<uint8>
   {
@@ -164,466 +117,557 @@ module MessageBody {
       SumPlaintextSegments(plaintextSeg[..|plaintextSeg| - 1]) + plaintextSeg[|plaintextSeg| - 1]
   }
 
-  lemma ExtendSumPlaintextSegments(plaintextSeg: seq<seq<uint8>>, plaintextFrame: seq<uint8>)
-    ensures SumPlaintextSegments(plaintextSeg + [plaintextFrame]) == SumPlaintextSegments(plaintextSeg) + plaintextFrame
+  // lemma ExtendSumPlaintextSegments(plaintextSeg: seq<seq<uint8>>, plaintextFrame: seq<uint8>)
+  //   ensures SumPlaintextSegments(plaintextSeg + [plaintextFrame]) == SumPlaintextSegments(plaintextSeg) + plaintextFrame
+  // {
+  // }
+
+  type FramedMessage = frames: seq<Frames.Frame>
+  |
+  // The total number of frames MUST be < UINT16_LENGTH
+  && 0 < |frames| <= ENDFRAME_SEQUENCE_NUMBER as nat
+  && var tail := Seq.Last(frames);
+  // The last element MUST be a final frame.
+  && Frames.IsFinalFrame(tail)
+  // All other frames MUST be RegularFrames
+  && (forall i
+    | 0 <= i < |Seq.DropLast(frames)|
+    :: Frames.IsRegularFrame(frames[i]))
+  && (forall i
+    | 0 <= i < |frames|
+    ::
+      // The sequence number MUST be monotonic
+      && frames[i].seqNum as nat == i + START_SEQUENCE_NUMBER as nat
+      // All frames MUST all be from the same messages with the same header
+      && frames[i].header == tail.header)
+  witness *
+
+
+  lemma asdf(
+    regularFrames: seq<Frames.RegularFrame>,
+    frame: Frames.RegularFrame
+  )
+    requires forall i // Sequence of frames is valid
+      | 0 <= i < |regularFrames|
+      :: regularFrames[i].seqNum as nat == i + START_SEQUENCE_NUMBER as nat
+    requires frame.seqNum as nat == |regularFrames| + START_SEQUENCE_NUMBER as nat
+    ensures forall i, frames : seq<Frames.RegularFrame>
+      |
+        && frames == regularFrames + [frame]
+        && 0 <= i < |frames|
+      :: frames[i].seqNum as nat == i + START_SEQUENCE_NUMBER as nat
   {
+
   }
 
-  datatype SeqWithGhostFrames = SeqWithGhostFrames(sequence: seq<uint8>, ghost frames: seq<Frame>)
+
 
   method EncryptMessageBody(
     plaintext: seq<uint8>,
-    frameLength: int,
-    messageID: Msg.MessageID,
-    key: seq<uint8>,
-    suite: Client.AlgorithmSuites.AlgorithmSuite
+    header : Header.Header,
+    key: seq<uint8>
   )
-    returns (result: Result<SeqWithGhostFrames, string>)
-    requires |key| ==  suite.encrypt.keyLength as int
-    requires 0 < frameLength < UINT32_LIMIT
+    returns (result: Result<seq<Frames.Frame>, string>)
+    requires |key| ==  header.suite.encrypt.keyLength as nat
+    requires 0 < header.body.frameLength as nat < UINT32_LIMIT
+    requires header.body.contentType.Framed?
     ensures match result
       case Failure(e) => true
-      case Success(seqWithGhostFrames) =>
-        var frames := seqWithGhostFrames.frames;
-        ValidFrames(frames)
-        && (forall frame | frame in frames :: frame.Valid())
-        && (forall frame: Frame | frame in frames :: |frame.iv| == suite.encrypt.ivLength as int)
-        && FramesToSequence(frames) == seqWithGhostFrames.sequence
+      case Success(frames) =>
+        // var frames := seqWithGhostFrames.frames;
+        // ValidFrames(frames)
+        // && (forall frame | frame in frames :: frame.Valid())
+        // && (forall frame: Frame | frame in frames :: |frame.iv| == suite.encrypt.ivLength as int)
+        // && FramesToSequence(frames) == seqWithGhostFrames.sequence
         && FramesEncryptPlaintext(frames, plaintext)
-        && (forall frame: Frame | frame in frames :: AESEncryption.EncryptedWithKey(frame.encContent, key))
+        && (forall frame: Frames.Frame | frame in frames :: AESEncryption.EncryptedWithKey(frame.encContent, key))
   {
-    var body := [];
+    // var body := [];
     var n : int, sequenceNumber := 0, START_SEQUENCE_NUMBER;
-    ghost var frames : seq<Frame> := [];
-    ghost var plaintextSeg := [];
+    var regularFrames: seq<Frames.RegularFrame> := [];
+    // ghost var plaintextSeg := [];
 
-    while n + frameLength < |plaintext|
+    while n + header.body.frameLength as nat < |plaintext|
       invariant |plaintext| != 0 ==> 0 <= n < |plaintext|
       invariant |plaintext| == 0 ==> 0 == n
+      // This needs to be inclusive
+      // because this invariant MUST also be true when the loop exists.
+      // If the final frame is going to be ENDFRAME_SEQUENCE_NUMBER,
+      // then when this loop exists, sequenceNumber == ENDFRAME_SEQUENCE_NUMBER.
       invariant START_SEQUENCE_NUMBER <= sequenceNumber <= ENDFRAME_SEQUENCE_NUMBER
-      invariant |frames| == (sequenceNumber - START_SEQUENCE_NUMBER) as int
-      invariant forall i | 0 <= i < |frames| :: // Sequence of frames is valid
-        var frame := frames[i];
-        frame.Valid() &&
-        frame.RegularFrame? &&
-        frame.seqNum as int == i + START_SEQUENCE_NUMBER as int
-      invariant forall i | 0 <= i < |frames| :: frames[i].iv == IVSeq(suite, frames[i].seqNum)
-      invariant FramesToSequence(frames) == body
-      invariant FramesEncryptPlaintextSegments(frames, plaintextSeg) // Frames decrypt to chunks of plaintext
-      invariant SumPlaintextSegments(plaintextSeg) == plaintext[..n] // Chunks of plaintext sum up to plaintexts
-      invariant forall frame: Frame | frame in frames :: AESEncryption.EncryptedWithKey(frame.encContent, key)
+      invariant |regularFrames| == (sequenceNumber - START_SEQUENCE_NUMBER) as nat
+      invariant forall i // Sequence of frames is valid
+      | 0 <= i < |regularFrames|
+      ::
+        && regularFrames[i].seqNum as nat == i + START_SEQUENCE_NUMBER as nat
+        && regularFrames[i].header == header
+      // invariant forall i | 0 <= i < |regularFrames| :: regularFrames[i].iv == IVSeq(suite, regularFrames[i].seqNum)
+      // invariant FramesToSequence(regularFrames) == body
+      // invariant FramesEncryptPlaintextSegments(regularFrames, plaintextSeg) // Frames decrypt to chunks of plaintext
+      // invariant SumPlaintextSegments(plaintextSeg) == plaintext[..n] // Chunks of plaintext sum up to plaintexts
+      invariant forall frame: Frames.Frame
+      | frame in regularFrames
+      :: AESEncryption.EncryptedWithKey(frame.encContent, key)
     {
-      assert {:split_here} true;
-      if sequenceNumber == ENDFRAME_SEQUENCE_NUMBER {
-        return Failure("too many frames");
-      }
-      var plaintextFrame := plaintext[n..n + frameLength];
-      var regularFrame, frame := EncryptRegularFrame(suite, key, frameLength, messageID, plaintextFrame, sequenceNumber);
-      if regularFrame.IsFailure() {
-        return regularFrame.PropagateFailure();
-      }
-      assert frame.iv == IVSeq(suite, sequenceNumber);
+      // assert {:split_here} true;
+      :- Need(sequenceNumber < ENDFRAME_SEQUENCE_NUMBER, "too many frames");
+      var plaintextFrame := plaintext[n..n + header.body.frameLength as nat];
+      var regularFrame :- EncryptRegularFrame(
+        key,
+        header,
+        plaintextFrame,
+        sequenceNumber
+      );
 
-      // Proofs that invariant holds after loop
-      ExtendFramesToSequence(frames, frame);
-      ExtendFramesEncryptPlaintextSegments(frames, plaintextSeg, frame, plaintextFrame);
-      ExtendSumPlaintextSegments(plaintextSeg, plaintextFrame);
-      frames := frames + [frame];
-      body := body + regularFrame.Extract();
-      plaintextSeg := plaintextSeg + [plaintextFrame];
+      asdf(regularFrames, regularFrame);
 
-      n, sequenceNumber := n + frameLength, sequenceNumber + 1;
-      assert SumPlaintextSegments(plaintextSeg) == plaintext[..n];
+      // assert frame.iv == IVSeq(suite, sequenceNumber);
+      // // Proofs that invariant holds after loop
+      // ExtendFramesToSequence(frames, frame);
+      // ExtendFramesEncryptPlaintextSegments(frames, plaintextSeg, frame, plaintextFrame);
+      // ExtendSumPlaintextSegments(plaintextSeg, plaintextFrame);
+      regularFrames := regularFrames + [regularFrame];
+      // body := body + regularFrame.Extract();
+      // plaintextSeg := plaintextSeg + [plaintextFrame];
+
+      n, sequenceNumber := n + header.body.frameLength as nat, sequenceNumber + 1;
+      // assert SumPlaintextSegments(plaintextSeg) == plaintext[..n];
     }
-    assert {:split_here} true;
+    // assert {:split_here} true;
 
-    var finalFrameResult, finalFrame := EncryptFinalFrame(suite, key, frameLength, messageID, plaintext[n..], sequenceNumber);
-    if finalFrameResult.IsFailure() {
-      return finalFrameResult.PropagateFailure();
-    }
-    var finalFrameSequence := finalFrameResult.Extract();
-    assert finalFrame.iv == IVSeq(suite, sequenceNumber);
-    ExtendFramesToSequence(frames, finalFrame);
-    ExtendFramesEncryptPlaintextSegments(frames, plaintextSeg, finalFrame, plaintext[n..]);
-    ExtendSumPlaintextSegments(plaintextSeg, plaintext[n..]);
-    frames := frames + [finalFrame];
-    body := body + finalFrameSequence;
-    plaintextSeg := plaintextSeg + [plaintext[n..]];
-    assert ValidFrames(frames) by {
-      forall i,j | 0 <= i < j < |frames|
-        ensures frames[i].iv != frames[j].iv
-      {
-        assert frames[i].seqNum as int == i + START_SEQUENCE_NUMBER as int;
-        assert frames[j].seqNum as int == j + START_SEQUENCE_NUMBER as int;
-        assert frames[i].iv == IVSeq(suite, frames[i].seqNum);
-        assert frames[j].iv == IVSeq(suite, frames[j].seqNum);
-        IVSeqDistinct(suite, frames[i].seqNum, frames[j].seqNum);
-      }
-    }
+    var finalFrame :- EncryptFinalFrame(
+      key,
+      header,
+      plaintext[n..],
+      sequenceNumber
+    );
 
-    result := Success(SeqWithGhostFrames(body, frames));
+    // var finalFrameSequence := finalFrameResult.Extract();
+    // assert finalFrame.iv == IVSeq(suite, sequenceNumber);
+    // ExtendFramesToSequence(frames, finalFrame);
+    // ExtendFramesEncryptPlaintextSegments(frames, plaintextSeg, finalFrame, plaintext[n..]);
+    // ExtendSumPlaintextSegments(plaintextSeg, plaintext[n..]);
+    var frames := regularFrames + [finalFrame];
+    // body := body + finalFrameSequence;
+    // plaintextSeg := plaintextSeg + [plaintext[n..]];
+    // assert ValidFrames(frames) by {
+    //   forall i,j | 0 <= i < j < |frames|
+    //     ensures frames[i].iv != frames[j].iv
+    //   {
+    //     assert frames[i].seqNum as int == i + START_SEQUENCE_NUMBER as int;
+    //     assert frames[j].seqNum as int == j + START_SEQUENCE_NUMBER as int;
+    //     assert frames[i].iv == IVSeq(suite, frames[i].seqNum);
+    //     assert frames[j].iv == IVSeq(suite, frames[j].seqNum);
+    //     IVSeqDistinct(suite, frames[i].seqNum, frames[j].seqNum);
+    //   }
+    // }
+
+    assert |frames| <= ENDFRAME_SEQUENCE_NUMBER as nat;
+    assert Frames.IsFinalFrame(Seq.Last(frames));
+    assert |frames| == (sequenceNumber - START_SEQUENCE_NUMBER + 1) as nat;
+    assert Seq.Last(frames).seqNum == sequenceNumber;
+    assert Seq.Last(frames).seqNum as nat == |frames|;
+    assert Seq.DropLast(frames) == regularFrames;
+    // assert forall i
+    // | 0 <= i < |Seq.DropLast(frames)|
+    // ::
+    //   // All other frames MUST be RegularFrames
+    //   && Frames.IsRegularFrame(frames[i])
+    //   // The sequence number MUST be monotonic
+    //   && frames[i].seqNum as nat == i + START_SEQUENCE_NUMBER as nat
+    //   // All frames MUST all be from the same messages with the same header
+    //   && frames[i].header == Seq.Last(frames).header;
+
+    return Success(frames);
   }
 
   method EncryptRegularFrame(
-    suite: Client.AlgorithmSuites.AlgorithmSuite,
     key: seq<uint8>,
-    ghost frameLength: int,
-    messageID: Msg.MessageID,
+    header: Header.Header,
     plaintext: seq<uint8>,
     sequenceNumber: uint32
   )
-    returns (res: Result<seq<uint8>, string>, ghost regFrame: Frame)
-    requires |key| == suite.encrypt.keyLength as int
-    requires 0 < frameLength < UINT32_LIMIT && START_SEQUENCE_NUMBER <= sequenceNumber <= ENDFRAME_SEQUENCE_NUMBER
+    returns (res: Result<Frames.RegularFrame, string>)
+    requires |key| == header.suite.encrypt.keyLength as int
+    requires 0 < header.body.frameLength as nat < UINT32_LIMIT && START_SEQUENCE_NUMBER <= sequenceNumber < ENDFRAME_SEQUENCE_NUMBER
+    requires header.body.contentType.Framed?
     requires |plaintext| < UINT32_LIMIT
-    requires |plaintext| == frameLength && sequenceNumber != ENDFRAME_SEQUENCE_NUMBER
+    requires |plaintext| == header.body.frameLength as nat && sequenceNumber != ENDFRAME_SEQUENCE_NUMBER
     // Why is this require here? ivLength is 12, not ever 4-11. ?
     // requires 4 <= suite.encrypt.ivLength as int
     ensures match res
       case Failure(e) => true
-      case Success(resultSuccess) =>
-           // Decrypt serialized frame back to frame and state that it is equal to the ghost frame
-        4 + suite.encrypt.ivLength as int + suite.encrypt.tagLength as int + frameLength == |resultSuccess|
-        && var iv := IVSeq(suite, sequenceNumber);
-        var encContent := resultSuccess[4 + suite.encrypt.ivLength as int..4 + suite.encrypt.ivLength as int + frameLength];
-        var authTag := resultSuccess[4 + suite.encrypt.ivLength as int + frameLength..];
-        var frame := RegularFrame(sequenceNumber, iv, encContent, authTag);
-        frame == regFrame
-        && FrameToSequence(regFrame) == resultSuccess
+      case Success(frame) =>
+        //    // Decrypt serialized frame back to frame and state that it is equal to the ghost frame
+        // 4 + suite.encrypt.ivLength as int + suite.encrypt.tagLength as int + frameLength == |resultSuccess|
+        // && var iv := IVSeq(suite, sequenceNumber);
+        // var encContent := resultSuccess[4 + suite.encrypt.ivLength as int..4 + suite.encrypt.ivLength as int + frameLength];
+        // var authTag := resultSuccess[4 + suite.encrypt.ivLength as int + frameLength..];
+        // var frame := RegularFrame(sequenceNumber, iv, encContent, authTag);
+        // frame == regFrame
+        // && FrameToSequence(regFrame) == resultSuccess
         && AESEncryption.CiphertextGeneratedWithPlaintext(frame.encContent, plaintext)
         && AESEncryption.EncryptedWithKey(frame.encContent, key)
+        && frame.seqNum == sequenceNumber
+        && frame.header == header
   {
     var seqNumSeq := UInt32ToSeq(sequenceNumber);
     var unauthenticatedFrame := seqNumSeq;
-    var iv := IVSeq(suite, sequenceNumber);
-    var aad := BodyAAD(messageID, AADRegularFrame, sequenceNumber, |plaintext| as uint64);
+    var iv := IVSeq(header.suite, sequenceNumber);
+    var aad := BodyAAD(
+      header.body.messageId,
+      AADRegularFrame,
+      sequenceNumber,
+      |plaintext| as uint64
+    );
 
-    var encryptionOutputResult := AESEncryption.AESEncrypt(suite.encrypt, iv, key, plaintext, aad);
-    if encryptionOutputResult.IsFailure() {
-      res := encryptionOutputResult.PropagateFailure();
-      regFrame := RegularFrame(0, [], [], []); // irrelevant value supplied for the sake of determinism
-      return;
-    }
-    var encryptionOutput := encryptionOutputResult.Extract();
-    ghost var frame := RegularFrame(sequenceNumber, iv, encryptionOutput.cipherText, encryptionOutput.authTag);
+    var encryptionOutput :- AESEncryption.AESEncrypt(
+      header.suite.encrypt,
+      iv,
+      key,
+      plaintext,
+      aad
+    );
 
-    SeqWithUInt32Suffix(iv, sequenceNumber as nat);  // this proves SeqToNat(iv) == sequenceNumber as nat
-    unauthenticatedFrame := unauthenticatedFrame + iv;
-    unauthenticatedFrame := unauthenticatedFrame + encryptionOutput.cipherText + encryptionOutput.authTag;
+    var frame: Frames.RegularFrame := Frames.Frame.RegularFrame(
+      header,
+      sequenceNumber,
+      iv,
+      encryptionOutput.cipherText,
+      encryptionOutput.authTag
+    );
 
-    return Success(unauthenticatedFrame), frame;
+    // SeqWithUInt32Suffix(iv, sequenceNumber as nat);  // this proves SeqToNat(iv) == sequenceNumber as nat
+    // unauthenticatedFrame := unauthenticatedFrame + iv;
+    // unauthenticatedFrame := unauthenticatedFrame + encryptionOutput.cipherText + encryptionOutput.authTag;
+
+    return Success(frame);
   }
 
   method EncryptFinalFrame(
-    suite: Client.AlgorithmSuites.AlgorithmSuite,
     key: seq<uint8>,
-    frameLength: int,
-    messageID: Msg.MessageID,
+    header: Header.Header,
     plaintext: seq<uint8>,
     sequenceNumber: uint32
   )
-    returns (res: Result<seq<uint8>, string>, ghost finalFrame: Frame)
-    requires |key| == suite.encrypt.keyLength as int
+    returns (res: Result<Frames.FinalFrame, string>)
+    requires |key| == header.suite.encrypt.keyLength as nat
     requires START_SEQUENCE_NUMBER <= sequenceNumber <= ENDFRAME_SEQUENCE_NUMBER
     requires 0 <= |plaintext| < UINT32_LIMIT
-    requires 0 < frameLength < UINT32_LIMIT
-    requires |plaintext| <= frameLength
-    requires 4 <= suite.encrypt.ivLength as int
+    // requires 0 < header.body.frameLength as nat < UINT32_LIMIT
+    requires header.body.contentType.Framed?
+    requires |plaintext| <= header.body.frameLength as nat
+    // requires 4 <= header.suite.encrypt.ivLength as int
     ensures match res
       case Failure(e) => true
-      case Success(resultSuccess) =>
-        // Decrypt serialized frame back to frame and state that it is equal to the ghost frame
-        4 + 4 + suite.encrypt.ivLength as int + 4 + suite.encrypt.tagLength as int <= |resultSuccess|
-          <= 4 + 4 + suite.encrypt.ivLength as int + 4 + suite.encrypt.tagLength as int + frameLength
-        && var contentLength : uint32 := SeqToUInt32(resultSuccess[4+4+suite.encrypt.ivLength as int..4+4+suite.encrypt.ivLength as int+4]);
-        |resultSuccess| == 4 + 4 + suite.encrypt.ivLength as int + 4 + contentLength as int + suite.encrypt.tagLength as int
-        && resultSuccess[..4] == UInt32ToSeq(ENDFRAME_SEQUENCE_NUMBER)
-        && |plaintext| == SeqToUInt32(resultSuccess[4 + 4 + suite.encrypt.ivLength as int..4 + 4 + suite.encrypt.ivLength as int + 4]) as int &&
-        var iv := IVSeq(suite, sequenceNumber);
-        var encContent := resultSuccess[4 + 4 + suite.encrypt.ivLength as int + 4..][..|plaintext|];
-        var authTag := resultSuccess[4 + 4 + suite.encrypt.ivLength as int + 4 + |plaintext|..];
-        var frame := FinalFrame(sequenceNumber, iv, encContent, authTag);
-        FrameToSequence(frame) == resultSuccess
-        && finalFrame == frame
+      case Success(frame) =>
+        // // Decrypt serialized frame back to frame and state that it is equal to the ghost frame
+        // 4 + 4 + suite.encrypt.ivLength as int + 4 + suite.encrypt.tagLength as int <= |resultSuccess|
+        //   <= 4 + 4 + suite.encrypt.ivLength as int + 4 + suite.encrypt.tagLength as int + frameLength
+        // && var contentLength : uint32 := SeqToUInt32(resultSuccess[4+4+suite.encrypt.ivLength as int..4+4+suite.encrypt.ivLength as int+4]);
+        // |resultSuccess| == 4 + 4 + suite.encrypt.ivLength as int + 4 + contentLength as int + suite.encrypt.tagLength as int
+        // && resultSuccess[..4] == UInt32ToSeq(ENDFRAME_SEQUENCE_NUMBER)
+        // && |plaintext| == SeqToUInt32(resultSuccess[4 + 4 + suite.encrypt.ivLength as int..4 + 4 + suite.encrypt.ivLength as int + 4]) as int &&
+        // var iv := IVSeq(suite, sequenceNumber);
+        // var encContent := resultSuccess[4 + 4 + suite.encrypt.ivLength as int + 4..][..|plaintext|];
+        // var authTag := resultSuccess[4 + 4 + suite.encrypt.ivLength as int + 4 + |plaintext|..];
+        // var frame := FinalFrame(sequenceNumber, iv, encContent, authTag);
+        // FrameToSequence(frame) == resultSuccess
+        // && finalFrame == frame
         && AESEncryption.CiphertextGeneratedWithPlaintext(frame.encContent, plaintext)
         && AESEncryption.EncryptedWithKey(frame.encContent, key)
+        && frame.seqNum == sequenceNumber
+        && frame.header == header
   {
-    var unauthenticatedFrame := UInt32ToSeq(ENDFRAME_SEQUENCE_NUMBER);
-    var seqNumSeq := UInt32ToSeq(sequenceNumber);
-    unauthenticatedFrame := unauthenticatedFrame + seqNumSeq;
+    // var unauthenticatedFrame := UInt32ToSeq(ENDFRAME_SEQUENCE_NUMBER);
+    // var seqNumSeq := UInt32ToSeq(sequenceNumber);
+    // unauthenticatedFrame := unauthenticatedFrame + seqNumSeq;
 
-    var iv := IVSeq(suite, sequenceNumber);
-    SeqWithUInt32Suffix(iv, sequenceNumber as nat);  // this proves SeqToNat(iv) == sequenceNumber as nat
-    unauthenticatedFrame := unauthenticatedFrame + iv;
-    unauthenticatedFrame := unauthenticatedFrame + UInt32ToSeq(|plaintext| as uint32);
+    var iv := IVSeq(header.suite, sequenceNumber);
+    // SeqWithUInt32Suffix(iv, sequenceNumber as nat);  // this proves SeqToNat(iv) == sequenceNumber as nat
+    // unauthenticatedFrame := unauthenticatedFrame + iv;
+    // unauthenticatedFrame := unauthenticatedFrame + UInt32ToSeq(|plaintext| as uint32);
 
-    var aad := BodyAAD(messageID, AADFinalFrame, sequenceNumber, |plaintext| as uint64);
+    var aad := BodyAAD(
+      header.body.messageId,
+      AADFinalFrame,
+      sequenceNumber,
+      |plaintext| as uint64
+    );
 
-    var encryptionOutputResult := AESEncryption.AESEncrypt(suite.encrypt, iv, key, plaintext, aad);
-    if encryptionOutputResult.IsFailure() {
-      res := encryptionOutputResult.PropagateFailure();
-      finalFrame := RegularFrame(0, [], [], []); // irrelevant value supplied for the sake of determinism
-      return;
-    }
-    var encryptionOutput := encryptionOutputResult.Extract();
-    unauthenticatedFrame := unauthenticatedFrame + encryptionOutput.cipherText + encryptionOutput.authTag;
-    assert |plaintext| == |encryptionOutput.cipherText|;
+    var encryptionOutput :- AESEncryption.AESEncrypt(
+      header.suite.encrypt,
+      iv,
+      key,
+      plaintext,
+      aad
+    );
 
-    ghost var frame := FinalFrame(sequenceNumber, iv, encryptionOutput.cipherText, encryptionOutput.authTag);
-    finalFrame := frame;
-    assert FrameToSequence(frame) == unauthenticatedFrame;
-    // Show which part of the serialized frame map to which frame variable
-    assert |plaintext| == SeqToUInt32(unauthenticatedFrame[4 + 4 + suite.encrypt.ivLength as int..4 + 4 + suite.encrypt.ivLength as int + 4]) as int;
-    assert |unauthenticatedFrame| == 4 + 4 + suite.encrypt.ivLength as int + 4 + |plaintext| + suite.encrypt.tagLength as int;
-    assert unauthenticatedFrame[4 + 4 + suite.encrypt.ivLength as int + 4..][..|plaintext|] == encryptionOutput.cipherText;
+    var finalFrame: Frames.FinalFrame := Frames.Frame.FinalFrame(
+      header,
+      sequenceNumber,
+      iv,
+      encryptionOutput.cipherText,
+      encryptionOutput.authTag
+    );
 
-    return Success(unauthenticatedFrame), finalFrame;
+    // var encryptionOutput := encryptionOutputResult.Extract();
+    // unauthenticatedFrame := unauthenticatedFrame + encryptionOutput.cipherText + encryptionOutput.authTag;
+    // assert |plaintext| == |encryptionOutput.cipherText|;
+
+    // ghost var frame := FinalFrame(sequenceNumber, iv, encryptionOutput.cipherText, encryptionOutput.authTag);
+    // finalFrame := frame;
+    // assert FrameToSequence(frame) == unauthenticatedFrame;
+    // // Show which part of the serialized frame map to which frame variable
+    // assert |plaintext| == SeqToUInt32(unauthenticatedFrame[4 + 4 + suite.encrypt.ivLength as int..4 + 4 + suite.encrypt.ivLength as int + 4]) as int;
+    // assert |unauthenticatedFrame| == 4 + 4 + suite.encrypt.ivLength as int + 4 + |plaintext| + suite.encrypt.tagLength as int;
+    // assert unauthenticatedFrame[4 + 4 + suite.encrypt.ivLength as int + 4..][..|plaintext|] == encryptionOutput.cipherText;
+
+    return Success(finalFrame);
   }
 
-  method DecryptFramedMessageBody(
-    rd: Streams.ByteReader,
-    suite: Client.AlgorithmSuites.AlgorithmSuite,
-    key: seq<uint8>,
-    frameLength: int,
-    messageID: Msg.MessageID
-  )
-    returns (res: Result<seq<uint8>, string>)
-    requires rd.Valid()
-    requires |key| == suite.encrypt.keyLength as int
-    requires 0 < frameLength < UINT32_LIMIT
-    modifies rd.reader`pos
-    ensures rd.Valid()
-    ensures res.Success? ==> DecryptedWithKey(key, res.value)
-    ensures match res
-      case Failure(_) => true
-      case Success(plaintext) => //Exists a sequence of frames which encrypts the plaintext and is serialized in the read section of the stream
-        old(rd.reader.pos) <= rd.reader.pos <= |rd.reader.data|
-        && exists frames: seq<Frame> | |frames| < UINT32_LIMIT && (forall frame | frame in frames :: frame.Valid())
-            && FramesToSequence(frames) == rd.reader.data[old(rd.reader.pos)..rd.reader.pos] ::
-              && FramesEncryptPlaintext(frames, plaintext)
-  {
-    var plaintext := [];
-    var n: uint32 := 1;
-    ghost var frames: seq<Frame> := [];
-    ghost var plaintextSeg: seq<seq<uint8>> := []; // Chuncks of plaintext which are decrypted from the frame
+  // method DecryptFramedMessageBody(
+  //   rd: Streams.ByteReader,
+  //   suite: Client.AlgorithmSuites.AlgorithmSuite,
+  //   key: seq<uint8>,
+  //   frameLength: int,
+  //   messageID: Msg.MessageID
+  // )
+  //   returns (res: Result<seq<uint8>, string>)
+  //   requires rd.Valid()
+  //   requires |key| == suite.encrypt.keyLength as int
+  //   requires 0 < frameLength < UINT32_LIMIT
+  //   modifies rd.reader`pos
+  //   ensures rd.Valid()
+  //   ensures res.Success? ==> DecryptedWithKey(key, res.value)
+  //   ensures match res
+  //     case Failure(_) => true
+  //     case Success(plaintext) => //Exists a sequence of frames which encrypts the plaintext and is serialized in the read section of the stream
+  //       old(rd.reader.pos) <= rd.reader.pos <= |rd.reader.data|
+  //       && exists frames: seq<Frame> | |frames| < UINT32_LIMIT && (forall frame | frame in frames :: frame.Valid())
+  //           && FramesToSequence(frames) == rd.reader.data[old(rd.reader.pos)..rd.reader.pos] ::
+  //             && FramesEncryptPlaintext(frames, plaintext)
+  // {
+  //   var plaintext := [];
+  //   var n: uint32 := 1;
+  //   ghost var frames: seq<Frame> := [];
+  //   ghost var plaintextSeg: seq<seq<uint8>> := []; // Chuncks of plaintext which are decrypted from the frame
 
-    while true
-      decreases ENDFRAME_SEQUENCE_NUMBER - n
-      invariant rd.Valid()
-      invariant n as int - 1 == |frames|
-      invariant n <= ENDFRAME_SEQUENCE_NUMBER
-      invariant forall frame | frame in frames :: frame.Valid()
-      invariant old(rd.reader.pos) <= rd.reader.pos <= |rd.reader.data|
-      invariant FramesToSequence(frames) == rd.reader.data[old(rd.reader.pos)..rd.reader.pos]
-      invariant rd.Valid()
-      invariant FramesEncryptPlaintextSegments(frames, plaintextSeg) // All decrypted frames decrypt to the list of plaintext chuncks
-      invariant SumPlaintextSegments(plaintextSeg) == plaintext // The current decrypted frame is the sum of all decrypted chuncks
-      invariant DecryptedSegmentsWithKey(key, plaintextSeg)
-      invariant plaintext == SumPlaintextSegments(plaintextSeg)
-    {
-      assert {:split_here} true;
-      var frameWithGhostSeq :- DecryptFrame(rd, suite, key, frameLength, messageID, n);
-      assert |frameWithGhostSeq.sequence| < UINT32_LIMIT;
-      var decryptedFrame := frameWithGhostSeq.frame;
-      ghost var ciphertext := frameWithGhostSeq.sequence;
-      assert |ciphertext| < UINT32_LIMIT;
-      ghost var encryptedFrame := if decryptedFrame.FinalFrame? then
-        FinalFrame(decryptedFrame.seqNum, decryptedFrame.iv, ciphertext, decryptedFrame.authTag)
-      else
-        RegularFrame(decryptedFrame.seqNum, decryptedFrame.iv, ciphertext, decryptedFrame.authTag);
-      assert encryptedFrame.Valid();
-      frames := frames + [encryptedFrame];
+  //   while true
+  //     decreases ENDFRAME_SEQUENCE_NUMBER - n
+  //     invariant rd.Valid()
+  //     invariant n as int - 1 == |frames|
+  //     invariant n <= ENDFRAME_SEQUENCE_NUMBER
+  //     invariant forall frame | frame in frames :: frame.Valid()
+  //     invariant old(rd.reader.pos) <= rd.reader.pos <= |rd.reader.data|
+  //     invariant FramesToSequence(frames) == rd.reader.data[old(rd.reader.pos)..rd.reader.pos]
+  //     invariant rd.Valid()
+  //     invariant FramesEncryptPlaintextSegments(frames, plaintextSeg) // All decrypted frames decrypt to the list of plaintext chuncks
+  //     invariant SumPlaintextSegments(plaintextSeg) == plaintext // The current decrypted frame is the sum of all decrypted chuncks
+  //     invariant DecryptedSegmentsWithKey(key, plaintextSeg)
+  //     invariant plaintext == SumPlaintextSegments(plaintextSeg)
+  //   {
+  //     assert {:split_here} true;
+  //     var frameWithGhostSeq :- DecryptFrame(rd, suite, key, frameLength, messageID, n);
+  //     assert |frameWithGhostSeq.sequence| < UINT32_LIMIT;
+  //     var decryptedFrame := frameWithGhostSeq.frame;
+  //     ghost var ciphertext := frameWithGhostSeq.sequence;
+  //     assert |ciphertext| < UINT32_LIMIT;
+  //     ghost var encryptedFrame := if decryptedFrame.FinalFrame? then
+  //       FinalFrame(decryptedFrame.seqNum, decryptedFrame.iv, ciphertext, decryptedFrame.authTag)
+  //     else
+  //       RegularFrame(decryptedFrame.seqNum, decryptedFrame.iv, ciphertext, decryptedFrame.authTag);
+  //     assert encryptedFrame.Valid();
+  //     frames := frames + [encryptedFrame];
 
-      var (decryptedFramePlaintext, final) := (decryptedFrame.encContent, decryptedFrame.FinalFrame?);
-      plaintext := plaintext + decryptedFramePlaintext;
-      plaintextSeg := plaintextSeg + [decryptedFramePlaintext];
-      if final {
-        assert FramesEncryptPlaintextSegments(frames, plaintextSeg);
-        assert SumPlaintextSegments(plaintextSeg) == plaintext;
-        break;
-      }
+  //     var (decryptedFramePlaintext, final) := (decryptedFrame.encContent, decryptedFrame.FinalFrame?);
+  //     plaintext := plaintext + decryptedFramePlaintext;
+  //     plaintextSeg := plaintextSeg + [decryptedFramePlaintext];
+  //     if final {
+  //       assert FramesEncryptPlaintextSegments(frames, plaintextSeg);
+  //       assert SumPlaintextSegments(plaintextSeg) == plaintext;
+  //       break;
+  //     }
 
-      n := n + 1;
-    }
-    assert |frames| < UINT32_LIMIT ;
-    assert (forall frame | frame in frames :: frame.Valid()) ;
-    assert FramesToSequence(frames) == rd.reader.data[old(rd.reader.pos)..rd.reader.pos];
-    return Success(plaintext);
-  }
+  //     n := n + 1;
+  //   }
+  //   assert |frames| < UINT32_LIMIT ;
+  //   assert (forall frame | frame in frames :: frame.Valid()) ;
+  //   assert FramesToSequence(frames) == rd.reader.data[old(rd.reader.pos)..rd.reader.pos];
+  //   return Success(plaintext);
+  // }
 
-  datatype FrameWithGhostSeq = FrameWithGhostSeq(frame: Frame, ghost sequence: seq<uint8>)
+  // method DecryptFrame(
+  //   rd: Streams.ByteReader,
+  //   suite: Client.AlgorithmSuites.AlgorithmSuite,
+  //   key: seq<uint8>,
+  //   frameLength: int,
+  //   messageID: Msg.MessageID,
+  //   expectedSequenceNumber: uint32
+  // )
+  //   returns (res: Result<FrameWithGhostSeq, string>)
+  //   requires rd.Valid()
+  //   requires |key| == suite.encrypt.keyLength as int
+  //   requires 0 < frameLength < UINT32_LIMIT
+  //   modifies rd.reader`pos
+  //   ensures rd.Valid()
+  //   ensures match res // If the expected sequence number is the end frame sequence number then the frame is the final frame. However, the final frame can arrive earlier
+  //     case Success(frameWithGhostSeq) =>
+  //       expectedSequenceNumber == ENDFRAME_SEQUENCE_NUMBER ==> frameWithGhostSeq.frame.FinalFrame?
+  //     case Failure(_) => true
+  //   ensures res.Success? ==> |res.value.sequence| < UINT32_LIMIT
+  //   ensures match res
+  //     case Success(frameWithGhostSeq) => ( // Decrypting the frame encoded in the stream is the returned ghost frame
+  //       && var decryptedFrame := frameWithGhostSeq.frame;
+  //          var ciphertext := frameWithGhostSeq.sequence;
+  //          var final := decryptedFrame.FinalFrame?;
+  //          decryptedFrame.Valid()
+  //       && old(rd.reader.pos) < rd.reader.pos <= |rd.reader.data|
+  //       && AESEncryption.CiphertextGeneratedWithPlaintext(ciphertext, decryptedFrame.encContent)
+  //       && AESEncryption.DecryptedWithKey(key, decryptedFrame.encContent)
+  //       && var encryptedFrame := (if decryptedFrame.FinalFrame? then
+  //            FinalFrame(decryptedFrame.seqNum, decryptedFrame.iv, ciphertext, decryptedFrame.authTag)
+  //          else
+  //            RegularFrame(decryptedFrame.seqNum, decryptedFrame.iv, ciphertext, decryptedFrame.authTag));
+  //          rd.reader.data[old(rd.reader.pos)..rd.reader.pos] == FrameToSequence(encryptedFrame)
+  //       && AESEncryption.CiphertextGeneratedWithPlaintext(encryptedFrame.encContent, decryptedFrame.encContent))
+  //     case Failure(_) => true
+  // {
+  //   var final := false;
+  //   var sequenceNumber :- rd.ReadUInt32();
+  //   ghost var frameSerialization := UInt32ToSeq(sequenceNumber);
+  //   assert rd.reader.data[old(rd.reader.pos)..rd.reader.pos] == frameSerialization;
 
-  method DecryptFrame(
-    rd: Streams.ByteReader,
-    suite: Client.AlgorithmSuites.AlgorithmSuite,
-    key: seq<uint8>,
-    frameLength: int,
-    messageID: Msg.MessageID,
-    expectedSequenceNumber: uint32
-  )
-    returns (res: Result<FrameWithGhostSeq, string>)
-    requires rd.Valid()
-    requires |key| == suite.encrypt.keyLength as int
-    requires 0 < frameLength < UINT32_LIMIT
-    modifies rd.reader`pos
-    ensures rd.Valid()
-    ensures match res // If the expected sequence number is the end frame sequence number then the frame is the final frame. However, the final frame can arrive earlier
-      case Success(frameWithGhostSeq) =>
-        expectedSequenceNumber == ENDFRAME_SEQUENCE_NUMBER ==> frameWithGhostSeq.frame.FinalFrame?
-      case Failure(_) => true
-    ensures res.Success? ==> |res.value.sequence| < UINT32_LIMIT
-    ensures match res
-      case Success(frameWithGhostSeq) => ( // Decrypting the frame encoded in the stream is the returned ghost frame
-        && var decryptedFrame := frameWithGhostSeq.frame;
-           var ciphertext := frameWithGhostSeq.sequence;
-           var final := decryptedFrame.FinalFrame?;
-           decryptedFrame.Valid()
-        && old(rd.reader.pos) < rd.reader.pos <= |rd.reader.data|
-        && AESEncryption.CiphertextGeneratedWithPlaintext(ciphertext, decryptedFrame.encContent)
-        && AESEncryption.DecryptedWithKey(key, decryptedFrame.encContent)
-        && var encryptedFrame := (if decryptedFrame.FinalFrame? then
-             FinalFrame(decryptedFrame.seqNum, decryptedFrame.iv, ciphertext, decryptedFrame.authTag)
-           else
-             RegularFrame(decryptedFrame.seqNum, decryptedFrame.iv, ciphertext, decryptedFrame.authTag));
-           rd.reader.data[old(rd.reader.pos)..rd.reader.pos] == FrameToSequence(encryptedFrame)
-        && AESEncryption.CiphertextGeneratedWithPlaintext(encryptedFrame.encContent, decryptedFrame.encContent))
-      case Failure(_) => true
-  {
-    var final := false;
-    var sequenceNumber :- rd.ReadUInt32();
-    ghost var frameSerialization := UInt32ToSeq(sequenceNumber);
-    assert rd.reader.data[old(rd.reader.pos)..rd.reader.pos] == frameSerialization;
+  //   if sequenceNumber == ENDFRAME_SEQUENCE_NUMBER {
+  //     final := true;
+  //     sequenceNumber :- rd.ReadUInt32();
+  //     frameSerialization := frameSerialization + UInt32ToSeq(sequenceNumber);
+  //     assert rd.reader.data[old(rd.reader.pos)..rd.reader.pos] == frameSerialization;
+  //   }
 
-    if sequenceNumber == ENDFRAME_SEQUENCE_NUMBER {
-      final := true;
-      sequenceNumber :- rd.ReadUInt32();
-      frameSerialization := frameSerialization + UInt32ToSeq(sequenceNumber);
-      assert rd.reader.data[old(rd.reader.pos)..rd.reader.pos] == frameSerialization;
-    }
+  //   if sequenceNumber != expectedSequenceNumber {
+  //     return Failure("unexpected frame sequence number");
+  //   }
 
-    if sequenceNumber != expectedSequenceNumber {
-      return Failure("unexpected frame sequence number");
-    }
+  //   assert {:focus} true;
+  //   var iv :- rd.ReadBytes(suite.encrypt.ivLength as int);
+  //   frameSerialization := frameSerialization + iv;
+  //   assert rd.reader.data[old(rd.reader.pos)..rd.reader.pos] == frameSerialization;
 
-    assert {:focus} true;
-    var iv :- rd.ReadBytes(suite.encrypt.ivLength as int);
-    frameSerialization := frameSerialization + iv;
-    assert rd.reader.data[old(rd.reader.pos)..rd.reader.pos] == frameSerialization;
+  //   var len := frameLength as uint32;
+  //   if final {
+  //     len :- rd.ReadUInt32();
+  //     if len > frameLength as uint32 {
+  //       return Failure("Final frame too long");
+  //     }
+  //     frameSerialization := frameSerialization + UInt32ToSeq(len);
+  //   }
 
-    var len := frameLength as uint32;
-    if final {
-      len :- rd.ReadUInt32();
-      if len > frameLength as uint32 {
-        return Failure("Final frame too long");
-      }
-      frameSerialization := frameSerialization + UInt32ToSeq(len);
-    }
+  //   var aad := BodyAAD(messageID, if final then AADFinalFrame else AADRegularFrame, sequenceNumber, len as uint64);
 
-    var aad := BodyAAD(messageID, if final then AADFinalFrame else AADRegularFrame, sequenceNumber, len as uint64);
+  //   assert {:focus} true;
+  //   var ciphertext :- rd.ReadBytes(len as nat);
+  //   frameSerialization := frameSerialization + ciphertext;
+  //   assert rd.reader.data[old(rd.reader.pos)..rd.reader.pos] == frameSerialization;
 
-    assert {:focus} true;
-    var ciphertext :- rd.ReadBytes(len as nat);
-    frameSerialization := frameSerialization + ciphertext;
-    assert rd.reader.data[old(rd.reader.pos)..rd.reader.pos] == frameSerialization;
+  //   var authTag :- rd.ReadBytes(suite.encrypt.tagLength as int);
+  //   frameSerialization := frameSerialization + authTag;
+  //   assert rd.reader.data[old(rd.reader.pos)..rd.reader.pos] == frameSerialization;
 
-    var authTag :- rd.ReadBytes(suite.encrypt.tagLength as int);
-    frameSerialization := frameSerialization + authTag;
-    assert rd.reader.data[old(rd.reader.pos)..rd.reader.pos] == frameSerialization;
+  //   var plaintext :- Decrypt(ciphertext, authTag, suite, iv, key, aad);
+  //   assert AESEncryption.CiphertextGeneratedWithPlaintext(ciphertext, plaintext);
+  //   assert rd.reader.data[old(rd.reader.pos)..rd.reader.pos] == frameSerialization;
 
-    var plaintext :- Decrypt(ciphertext, authTag, suite, iv, key, aad);
-    assert AESEncryption.CiphertextGeneratedWithPlaintext(ciphertext, plaintext);
-    assert rd.reader.data[old(rd.reader.pos)..rd.reader.pos] == frameSerialization;
+  //   var frame := if final then
+  //       FinalFrame(sequenceNumber, iv, plaintext, authTag)
+  //     else
+  //       RegularFrame(sequenceNumber, iv, plaintext, authTag);
 
-    var frame := if final then
-        FinalFrame(sequenceNumber, iv, plaintext, authTag)
-      else
-        RegularFrame(sequenceNumber, iv, plaintext, authTag);
+  //   ghost var encryptedFrame := if final then
+  //       FinalFrame(sequenceNumber, iv, ciphertext, authTag)
+  //     else
+  //       RegularFrame(sequenceNumber, iv, ciphertext, authTag);
 
-    ghost var encryptedFrame := if final then
-        FinalFrame(sequenceNumber, iv, ciphertext, authTag)
-      else
-        RegularFrame(sequenceNumber, iv, ciphertext, authTag);
+  //   // Feed dafny facts about the content of the stream
+  //   // Show dafny that the serialized frame is frameSerialization
+  //   assert frameSerialization == FrameToSequence(encryptedFrame);
 
-    // Feed dafny facts about the content of the stream
-    // Show dafny that the serialized frame is frameSerialization
-    assert frameSerialization == FrameToSequence(encryptedFrame);
+  //   // Prove read content of stream is frameSerialization
+  //   assert {:focus} true;
+  //   assert !final ==> frameSerialization[..4] == rd.reader.data[old(rd.reader.pos)..][..4];
+  //   assert !final ==> frameSerialization[4..][..suite.encrypt.ivLength as int] == rd.reader.data[old(rd.reader.pos)..][4..][..suite.encrypt.ivLength as int];
+  //   assert !final ==> frameSerialization[4 + suite.encrypt.ivLength as int..][..frameLength] == rd.reader.data[old(rd.reader.pos)..][4 + suite.encrypt.ivLength as int..][..frameLength];
+  //   assert !final ==> frameSerialization[4 + frameLength + suite.encrypt.ivLength as int..] == rd.reader.data[old(rd.reader.pos)..][4 + frameLength + suite.encrypt.ivLength as int..][..suite.encrypt.tagLength as int];
 
-    // Prove read content of stream is frameSerialization
-    assert {:focus} true;
-    assert !final ==> frameSerialization[..4] == rd.reader.data[old(rd.reader.pos)..][..4];
-    assert !final ==> frameSerialization[4..][..suite.encrypt.ivLength as int] == rd.reader.data[old(rd.reader.pos)..][4..][..suite.encrypt.ivLength as int];
-    assert !final ==> frameSerialization[4 + suite.encrypt.ivLength as int..][..frameLength] == rd.reader.data[old(rd.reader.pos)..][4 + suite.encrypt.ivLength as int..][..frameLength];
-    assert !final ==> frameSerialization[4 + frameLength + suite.encrypt.ivLength as int..] == rd.reader.data[old(rd.reader.pos)..][4 + frameLength + suite.encrypt.ivLength as int..][..suite.encrypt.tagLength as int];
+  //   // Prove equivalence frameSerialization and content read on the stream
+  //   assert rd.reader.data[old(rd.reader.pos)..rd.reader.pos] == frameSerialization;
 
-    // Prove equivalence frameSerialization and content read on the stream
-    assert rd.reader.data[old(rd.reader.pos)..rd.reader.pos] == frameSerialization;
+  //   assert old(rd.reader.pos) < rd.reader.pos <= |rd.reader.data|;
 
-    assert old(rd.reader.pos) < rd.reader.pos <= |rd.reader.data|;
-
-    return Success(FrameWithGhostSeq(frame,ciphertext));
-  }
+  //   return Success(FrameWithGhostSeq(frame,ciphertext));
+  // }
 
   method BodyAAD(messageID: seq<uint8>, bc: BodyAADContent, sequenceNumber: uint32, length: uint64) returns (aad: seq<uint8>) {
     var contentAAD := UTF8.Encode(BodyAADContentTypeString(bc));
     aad := messageID + contentAAD.value + UInt32ToSeq(sequenceNumber) + UInt64ToSeq(length);
   }
 
-  method Decrypt(
-    ciphertext: seq<uint8>,
-    authTag: seq<uint8>,
-    suite: Client.AlgorithmSuites.AlgorithmSuite,
-    iv: seq<uint8>,
-    key: seq<uint8>,
-    aad: seq<uint8>
-  )
-    returns (res: Result<seq<uint8>, string>)
-    requires 
-      && |iv| == suite.encrypt.ivLength as int
-      && |key| == suite.encrypt.keyLength as int
-      && |authTag| == suite.encrypt.tagLength as int
-    ensures res.Success? ==> AESEncryption.CiphertextGeneratedWithPlaintext(ciphertext, res.value)
-    ensures res.Success? ==> |ciphertext| == |res.value|
-    ensures res.Success? ==> AESEncryption.DecryptedWithKey(key, res.value)
-  {
-    var encAlg := suite.encrypt;
-    res := AESEncryption.AESDecrypt(encAlg, key, ciphertext, authTag, iv, aad);
-    assert res.Success? ==> AESEncryption.DecryptedWithKey(key, res.value);
-  }
+  // method Decrypt(
+  //   ciphertext: seq<uint8>,
+  //   authTag: seq<uint8>,
+  //   suite: Client.AlgorithmSuites.AlgorithmSuite,
+  //   iv: seq<uint8>,
+  //   key: seq<uint8>,
+  //   aad: seq<uint8>
+  // )
+  //   returns (res: Result<seq<uint8>, string>)
+  //   requires
+  //     && |iv| == suite.encrypt.ivLength as int
+  //     && |key| == suite.encrypt.keyLength as int
+  //     && |authTag| == suite.encrypt.tagLength as int
+  //   ensures res.Success? ==> AESEncryption.CiphertextGeneratedWithPlaintext(ciphertext, res.value)
+  //   ensures res.Success? ==> |ciphertext| == |res.value|
+  //   ensures res.Success? ==> AESEncryption.DecryptedWithKey(key, res.value)
+  // {
+  //   var encAlg := suite.encrypt;
+  //   res := AESEncryption.AESDecrypt(encAlg, key, ciphertext, authTag, iv, aad);
+  //   assert res.Success? ==> AESEncryption.DecryptedWithKey(key, res.value);
+  // }
 
-  predicate DecryptedWithKey(key: seq<uint8>, plaintext: seq<uint8>)
-  {
-    if AESEncryption.DecryptedWithKey(key, plaintext) then true else
-      exists plaintextSeg | SumPlaintextSegments(plaintextSeg) == plaintext ::
-        DecryptedSegmentsWithKey(key, plaintextSeg)
-  }
+  // predicate DecryptedWithKey(key: seq<uint8>, plaintext: seq<uint8>)
+  // {
+  //   if AESEncryption.DecryptedWithKey(key, plaintext) then true else
+  //     exists plaintextSeg | SumPlaintextSegments(plaintextSeg) == plaintext ::
+  //       DecryptedSegmentsWithKey(key, plaintextSeg)
+  // }
 
-  predicate DecryptedSegmentsWithKey(key: seq<uint8>, plaintextSeg: seq<seq<uint8>>)
-  {
-    if plaintextSeg == [] then true else
-      && DecryptedSegmentsWithKey(key, plaintextSeg[..|plaintextSeg| - 1])
-      && AESEncryption.DecryptedWithKey(key, plaintextSeg[|plaintextSeg| - 1])
-  }
+  // predicate DecryptedSegmentsWithKey(key: seq<uint8>, plaintextSeg: seq<seq<uint8>>)
+  // {
+  //   if plaintextSeg == [] then true else
+  //     && DecryptedSegmentsWithKey(key, plaintextSeg[..|plaintextSeg| - 1])
+  //     && AESEncryption.DecryptedWithKey(key, plaintextSeg[|plaintextSeg| - 1])
+  // }
 
-  method DecryptNonFramedMessageBody(
-    rd: Streams.ByteReader,
-    suite: Client.AlgorithmSuites.AlgorithmSuite,
-    key: seq<uint8>,
-    messageID: Msg.MessageID
-  )
-    returns (res: Result<seq<uint8>, string>)
-    requires rd.Valid()
-    requires |key| == suite.encrypt.keyLength as int
-    modifies rd.reader`pos
-    ensures rd.Valid()
-  {
-    var iv :- rd.ReadBytes(suite.encrypt.ivLength as int);
-    var contentLength :- rd.ReadUInt64();
-    var ciphertext :- rd.ReadBytes(contentLength as nat);
-    var authTag :- rd.ReadBytes(suite.encrypt.tagLength as int);
+  // method DecryptNonFramedMessageBody(
+  //   rd: Streams.ByteReader,
+  //   suite: Client.AlgorithmSuites.AlgorithmSuite,
+  //   key: seq<uint8>,
+  //   messageID: Msg.MessageID
+  // )
+  //   returns (res: Result<seq<uint8>, string>)
+  //   requires rd.Valid()
+  //   requires |key| == suite.encrypt.keyLength as int
+  //   modifies rd.reader`pos
+  //   ensures rd.Valid()
+  // {
+  //   var iv :- rd.ReadBytes(suite.encrypt.ivLength as int);
+  //   var contentLength :- rd.ReadUInt64();
+  //   var ciphertext :- rd.ReadBytes(contentLength as nat);
+  //   var authTag :- rd.ReadBytes(suite.encrypt.tagLength as int);
 
-    var aad := BodyAAD(messageID, AADSingleBlock, NONFRAMED_SEQUENCE_NUMBER, contentLength);
+  //   var aad := BodyAAD(messageID, AADSingleBlock, NONFRAMED_SEQUENCE_NUMBER, contentLength);
 
-    var plaintext :- Decrypt(ciphertext, authTag, suite, iv, key, aad);
-    return Success(plaintext);
-  }
+  //   var plaintext :- Decrypt(ciphertext, authTag, suite, iv, key, aad);
+  //   return Success(plaintext);
+  // }
 }
